A little more work on type checking

02Typed/Typechecking.thy
@@ -1,5 +1,5 @@
 theory Typechecking
-  imports Typed "../01Source/Named" "../00Utils/Unification/Unification"
+  imports Typed "../01Source/Named" UnifiableType
 begin
 
 datatype hexpr = 
@@ -26,9 +26,6 @@ primrec htvars :: "hexpr \<Rightarrow> var set" where
 | "htvars (HLam x t e) = vars t \<union> htvars e"
 | "htvars (HApp e\<^sub>1 e\<^sub>2) = htvars e\<^sub>1 \<union> htvars e\<^sub>2"
 
-definition env_subst :: "subst \<Rightarrow> subst \<Rightarrow> subst" where
-  "env_subst sub \<Gamma> = map_option (subst sub) \<circ> \<Gamma>"
-
 primrec typecheck' :: "subst \<Rightarrow> var set \<Rightarrow> nexpr \<Rightarrow> hexpr \<times> uexpr \<times> var set \<times> (uexpr \<times> uexpr) list" 
     where
   "typecheck' \<Gamma> vs (NVar x) = (case \<Gamma> x of 
@@ -45,28 +42,17 @@ primrec typecheck' :: "subst \<Rightarrow> var set \<Rightarrow> nexpr \<Rightar
     in let (e\<^sub>2', t\<^sub>2, vs'', con\<^sub>2) = typecheck' \<Gamma> vs' e\<^sub>2 
     in (HApp e\<^sub>1' e\<^sub>2', Var v, vs'', con\<^sub>1 @ con\<^sub>2 @ [(t\<^sub>1, Ctor ''Arrow'' [t\<^sub>2, Var v])]))"
 
-fun typeify :: "uexpr \<Rightarrow> ty" where
-  "typeify (Var v) = TyVar v"
-| "typeify (Ctor k []) = (if k = ''Base'' then Base else undefined)"
-| "typeify (Ctor k [t\<^sub>1, t\<^sub>2]) = 
-    (if k = ''Arrow'' then Arrow (typeify t\<^sub>1) (typeify t\<^sub>2) else undefined)"
-| "typeify (Ctor k ts) = undefined"
-
-primrec untypify :: "ty \<Rightarrow> uexpr" where
-  "untypify (TyVar v) = Var v"
-| "untypify Base = Ctor ''Base'' []"
-| "untypify (Arrow t\<^sub>1 t\<^sub>2) = Ctor ''Arrow'' [untypify t\<^sub>1, untypify t\<^sub>2]"
-
 primrec solidify :: "hexpr \<Rightarrow> texpr" where
   "solidify (HVar x) = TVar x"
 | "solidify (HConst k) = TConst k"
 | "solidify (HLam x t e) = TLam x (typeify t) (solidify e)"
 | "solidify (HApp e\<^sub>1 e\<^sub>2) = TApp (solidify e\<^sub>1) (solidify e\<^sub>2)"
 
-fun tsubsts :: "subst \<Rightarrow> ty \<Rightarrow> ty" where
-  "tsubsts sub (TyVar y) = (case sub y of Some t \<Rightarrow> typeify t | None \<Rightarrow> TyVar y)"
-| "tsubsts sub Base = Base"
-| "tsubsts sub (Arrow t\<^sub>1 t\<^sub>2) = Arrow (tsubsts sub t\<^sub>1) (tsubsts sub t\<^sub>2)"
+primrec liquify :: "texpr \<Rightarrow> hexpr" where
+  "liquify (TVar x) = HVar x"
+| "liquify (TConst k) = HConst k"
+| "liquify (TLam x t e) = HLam x (untypeify t) (liquify e)"
+| "liquify (TApp e\<^sub>1 e\<^sub>2) = HApp (liquify e\<^sub>1) (liquify e\<^sub>2)"
 
 primrec tsubstt :: "subst \<Rightarrow> texpr \<Rightarrow> texpr" where
   "tsubstt sub (TVar x) = TVar x"
@@ -80,22 +66,6 @@ fun typecheck :: "nexpr \<rightharpoonup> texpr \<times> ty" where
     in case unify' con of 
         Some sub \<Rightarrow> Some (tsubstt sub (solidify e'), tsubsts sub (typeify t))
       | None \<Rightarrow> None)"
-
-fun valid_ty_uexpr' :: "string \<Rightarrow> nat \<Rightarrow> bool" where
-  "valid_ty_uexpr' k 0 = (k = ''Base'')"
-| "valid_ty_uexpr' k (Suc 0) = False"
-| "valid_ty_uexpr' k (Suc (Suc 0)) = (k = ''Arrow'')"
-| "valid_ty_uexpr' k (Suc (Suc (Suc x))) = False"
-
-primrec valid_ty_uexpr :: "uexpr \<Rightarrow> bool" where
-  "valid_ty_uexpr (Var v) = True"
-| "valid_ty_uexpr (Ctor k ts) = (valid_ty_uexpr' k (length ts) \<and> list_all valid_ty_uexpr ts)"
-
-definition valid_ty_uexprs :: "(uexpr \<times> uexpr) list \<Rightarrow> bool" where
-  "valid_ty_uexprs ts = list_all (\<lambda>(t\<^sub>1, t\<^sub>2). valid_ty_uexpr t\<^sub>1 \<and> valid_ty_uexpr t\<^sub>2) ts"
- 
-definition valid_ty_subst :: "subst \<Rightarrow> bool" where
-  "valid_ty_subst \<Gamma> = (\<forall>t \<in> ran \<Gamma>. valid_ty_uexpr t)"
 
 primrec valid_ty_hexpr :: "hexpr \<Rightarrow> bool" where
   "valid_ty_hexpr (HVar x) = True"
@@ -120,55 +90,28 @@ lemma typecheck_induct [consumes 1, case_names NVarS NVarN NConst NLam NApp]: "
   by (induction e arbitrary: \<Gamma> vs e' t vs' con) 
      (auto simp add: Let_def split: option.splits prod.splits)
 
-lemma [simp]: "typeify (untypify t) = t"
-  by (induction t) simp_all
-
-lemma [simp]: "valid_ty_uexpr t \<Longrightarrow> untypify (typeify t) = t"
-  by (induction t rule: typeify.induct) simp_all
-
-lemma [dest]: "typeify e = Arrow t\<^sub>1 t\<^sub>2 \<Longrightarrow> valid_ty_uexpr e \<Longrightarrow> 
-    e = Ctor ''Arrow'' [untypify t\<^sub>1, untypify t\<^sub>2]"
-  by (induction e rule: typeify.induct) auto
-
-lemma [simp]: "vars (untypify t) = tvars t"
-  by (induction t) simp_all
-
-lemma [simp]: "valid_ty_uexpr (untypify t)"
-  by (induction t) simp_all
-
-lemma [simp]: "valid_ty_uexpr t \<Longrightarrow> tvars (typeify t) = vars t"
-  by (induction t rule: typeify.induct) simp_all
-
-lemma [simp]: "tsubsts Map.empty e = e"
+lemma [simp]: "valid_ty_hexpr (liquify e)"
   by (induction e) simp_all
-
-lemma [simp]: "dom s \<inter> tvars t = {} \<Longrightarrow> tsubsts s t = t"
-  by (induction t) (auto split: option.splits)
-
-lemma [simp]: "valid_ty_uexpr t \<Longrightarrow> typeify (subst sub t) = tsubsts sub (typeify t)"
-  by (induction t rule: typeify.induct) (simp_all split: option.splits)
 
 lemma [simp]: "x \<notin> htvars e \<Longrightarrow> hsubst [x \<mapsto> t] e = e"
   by (induction e) simp_all
 
-lemma hsubst_merge: "hsubst (extend_subst x t s) e = hsubst s (hsubst [x \<mapsto> t] e)"
+lemma [simp]: "hsubst (extend_subst x t s) e = hsubst s (hsubst [x \<mapsto> t] e)"
   by (induction e) (simp_all only: hsubst.simps subst_merge)
 
-lemma valid_empty [simp]: "valid_ty_subst Map.empty"
-  by (simp add: valid_ty_subst_def)
-
-lemma [simp]: "valid_ty_uexpr e \<Longrightarrow> typeify (subst sub e) = tsubsts sub (typeify e)"
-  by (induction e rule: typeify.induct) (auto split: option.splits)
-
-lemma [simp]: "valid_ty_subst \<Gamma> \<Longrightarrow> 
-    map_option (typeify \<circ> subst sub) (\<Gamma> x) = map_option (tsubsts sub \<circ> typeify) (\<Gamma> x)"
-  by (cases "\<Gamma> x") (auto simp add: valid_ty_subst_def ran_def)
-
-lemma [simp]: "valid_ty_subst \<Gamma> \<Longrightarrow> 
-    map_option (typeify \<circ> subst sub) \<circ> \<Gamma> = map_option (tsubsts sub \<circ> typeify) \<circ> \<Gamma>"
-  by auto
-
 lemma [simp]: "valid_ty_hexpr e \<Longrightarrow> solidify (hsubst sub e) = tsubstt sub (solidify e)"
+  by (induction e) simp_all
+
+lemma [simp]: "valid_ty_subst sub \<Longrightarrow> liquify (tsubstt sub e) = hsubst sub (liquify e)"
+  by (induction e) simp_all
+
+lemma [simp]: "solidify (liquify e) = e"
+  by (induction e) simp_all
+
+lemma [simp]: "valid_ty_hexpr e \<Longrightarrow> liquify (solidify e) = e"
+  by (induction e) simp_all
+
+lemma [simp]: "valid_ty_hexpr e \<Longrightarrow> tvarst (solidify e) = htvars e"
   by (induction e) simp_all
 
 lemma [simp]: "erase (solidify (hsubst sub e)) = erase (solidify e)"
@@ -177,93 +120,29 @@ lemma [simp]: "erase (solidify (hsubst sub e)) = erase (solidify e)"
 lemma [simp]: "erase (tsubstt sub e) = erase e"
   by (induction e) simp_all
 
-lemma [simp]: "valid_ty_subst \<Gamma> \<Longrightarrow> valid_ty_uexpr t \<Longrightarrow> valid_ty_subst (\<Gamma>(x \<mapsto> t))"
-  by (auto simp add: valid_ty_subst_def ran_def)
-
-lemma [simp]: "valid_ty_subst \<Gamma> \<Longrightarrow> valid_ty_subst \<Gamma>' \<Longrightarrow> valid_ty_subst (\<Gamma>(x := \<Gamma>' y))"
-  by (auto simp add: valid_ty_subst_def ran_def)
-
-lemma [simp]: "valid_ty_uexpr e \<Longrightarrow> valid_ty_uexpr e' \<Longrightarrow> valid_ty_uexpr (subst [x \<mapsto> e'] e)"
-  and [simp]: "list_all valid_ty_uexpr es \<Longrightarrow> valid_ty_uexpr e' \<Longrightarrow> 
-    list_all valid_ty_uexpr (map (subst [x \<mapsto> e']) es)"
-proof (induction e and es rule: vars_varss.induct)
-  case (2 k es)
-  thus ?case 
-  proof (induction es)
-    case (Cons a es)
-    thus ?case 
-    proof (induction es)
-      case (Cons b es)
-      thus ?case by (induction es) simp_all
-    qed simp_all
-  qed simp_all
-qed simp_all
-
-lemma [simp]: "valid_ty_uexpr e \<Longrightarrow> valid_ty_uexprs ess \<Longrightarrow> valid_ty_uexprs (list_subst x e ess)"
-  by (induction ess rule: list_subst.induct) (auto simp add: valid_ty_uexprs_def)
-
-lemma [simp]: "valid_ty_uexpr t \<Longrightarrow> valid_ty_subst sub \<Longrightarrow> valid_ty_uexpr (subst sub t)"
-  and [simp]: "list_all valid_ty_uexpr ts \<Longrightarrow> valid_ty_subst sub \<Longrightarrow> 
-    list_all valid_ty_uexpr (map (subst sub) ts)"
-  by (induction t and ts rule: vars_varss.induct) 
-     (auto simp add: valid_ty_subst_def ran_def split: option.splits)
-
-lemma [simp]: "valid_ty_subst (extend_subst x e s) = (valid_ty_uexpr e \<and> valid_ty_subst s)"
-  by (auto simp add: valid_ty_subst_def extend_subst_def ran_def)
-
-lemma [elim]: "valid_ty_subst \<Gamma> \<Longrightarrow> \<Gamma> x = Some t \<Longrightarrow> valid_ty_uexpr t"
-  by (auto simp add: valid_ty_subst_def ran_def)
-
-lemma [simp]: "valid_ty_subst \<Gamma> \<Longrightarrow> valid_ty_subst sub\<^sub>2 \<Longrightarrow> 
-  map_option (typeify \<circ> subst sub\<^sub>1 \<circ> subst sub\<^sub>2) (\<Gamma> x) = 
-    map_option (tsubsts sub\<^sub>1 \<circ> tsubsts sub\<^sub>2 \<circ> typeify) (\<Gamma> x)"
-proof (cases "\<Gamma> x")
-  case (Some e)
-  moreover assume "valid_ty_subst \<Gamma>"
-  ultimately have E: "valid_ty_uexpr e" by auto
-  assume "valid_ty_subst sub\<^sub>2"
-  with Some E show ?thesis by simp
-qed simp_all
-
-lemma [simp]: "valid_ty_subst \<Gamma> \<Longrightarrow> valid_ty_subst sub\<^sub>2 \<Longrightarrow> 
-  map_option (typeify \<circ> subst sub\<^sub>1 \<circ> subst sub\<^sub>2) \<circ> \<Gamma> = 
-    map_option (tsubsts sub\<^sub>1 \<circ> tsubsts sub\<^sub>2 \<circ> typeify) \<circ> \<Gamma>"
-  by auto
-
-lemma [elim]: "valid_ty_uexprs ts \<Longrightarrow> unify' ts = Some sub \<Longrightarrow> valid_ty_subst sub"                                  
-proof (induction ts arbitrary: sub rule: unify'.induct)
-  case (2 k\<^sub>1 es\<^sub>1 k\<^sub>2 es\<^sub>2 ess)
-  moreover hence "list_all valid_ty_uexpr es\<^sub>1" by (auto simp add: valid_ty_uexprs_def)
-  moreover from 2 have "list_all valid_ty_uexpr es\<^sub>2" by (auto simp add: valid_ty_uexprs_def)
-  ultimately show ?case by (simp add: valid_ty_uexprs_def split: if_splits)
-next
-  case (4 x e ess)
-  thus ?case
-  proof (cases "e = Var x")
-    case False note F = False
-    with 4 show ?thesis 
-    proof (cases "x \<in> vars e")
-      case False
-      with 4 F obtain sub' where S: "unify' (list_subst x e ess) = Some sub' \<and> 
-        sub = extend_subst x e sub'" by auto
-      from 4 have "valid_ty_uexpr e \<and> valid_ty_uexprs ess" by (simp add: valid_ty_uexprs_def)
-      hence "valid_ty_uexprs (list_subst x e ess)" by simp
-      with 4 F False S show ?thesis by (simp add: valid_ty_uexprs_def)
-    qed simp_all
-  qed (simp_all add: valid_ty_uexprs_def)
-qed (auto simp add: valid_ty_uexprs_def)
-
-lemma [elim]: "valid_ty_uexpr t\<^sub>1 \<Longrightarrow> valid_ty_uexpr t\<^sub>2 \<Longrightarrow> unify t\<^sub>1 t\<^sub>2 = Some sub \<Longrightarrow> 
-  valid_ty_subst sub"                                  
-proof (unfold unify_def)
-  assume "valid_ty_uexpr t\<^sub>1" and "valid_ty_uexpr t\<^sub>2" 
-  hence "valid_ty_uexprs [(t\<^sub>1, t\<^sub>2)]" by (simp add: valid_ty_uexprs_def)
-  moreover assume "unify' [(t\<^sub>1, t\<^sub>2)] = Some sub"
-  ultimately show "valid_ty_subst sub" by auto
-qed
-
 lemma [simp]: "valid_ty_subst sub \<Longrightarrow> valid_ty_hexpr e \<Longrightarrow> valid_ty_hexpr (hsubst sub e)"
   by (induction e) simp_all
+
+lemma [simp]: "htvars (hsubst sub e) \<subseteq> htvars e - dom sub \<union> subst_vars sub"
+proof (induction e)
+  case (HLam x t e)
+  moreover have "vars (subst sub t) \<subseteq> vars t - dom sub \<union> subst_vars sub" by simp
+  ultimately show ?case by fastforce
+qed auto
+
+lemma [simp]: "dom sub \<inter> htvars e = {} \<Longrightarrow> hsubst sub e = e"
+proof (induction e)
+  case (HLam x t e)
+  moreover hence "dom sub \<inter> vars t = {}" by auto
+  ultimately show ?case by auto
+qed auto
+
+lemma [simp]: "dom sub \<inter> tvarst e = {} \<Longrightarrow> tsubstt sub e = e"
+proof (induction e)
+  case (TLam x t e)
+  moreover hence "dom sub \<inter> tvars t = {}" by auto
+  ultimately show ?case by auto
+qed auto
 
 lemma tc_tsubstt [simp]: "\<Gamma> \<turnstile>\<^sub>n e : t \<Longrightarrow> 
   map_option (tsubsts sub) \<circ> \<Gamma> \<turnstile>\<^sub>n tsubstt sub e : tsubsts sub t"
@@ -274,28 +153,6 @@ proof (induction \<Gamma> e t rule: typecheckn.induct)
     by simp
   thus ?case by blast
 qed simp_all
-
-lemma valid_ty_uexpr_structrual [simp]: "structural valid_ty_uexpr"
-  by (auto simp add: structural_def)
-
-lemma [simp]: "valid_ty_subst sub \<Longrightarrow> valid_ty_subst \<Gamma> \<Longrightarrow> valid_ty_subst (env_subst sub \<Gamma>)"
-  by (auto simp add: valid_ty_subst_def env_subst_def ran_def)
-
-lemma [simp]: "valid_ty_subst s1 \<Longrightarrow> valid_ty_subst s2 \<Longrightarrow> valid_ty_subst (combine_subst s1 s2)"
-proof (unfold valid_ty_subst_def combine_subst_def ran_def, rule)
-  fix x
-  assume S1: "\<forall>x \<in> {b. \<exists>a. s1 a = Some b}. valid_ty_uexpr x"
-  assume S2: "\<forall>x \<in> {b. \<exists>a. s2 a = Some b}. valid_ty_uexpr x"
-  assume "x \<in> {b. \<exists>a. (case s2 a of None \<Rightarrow> s1 a | Some e \<Rightarrow> Some (subst s1 e)) = Some b}"
-  then obtain y where Y: "(case s2 y of None \<Rightarrow> s1 y | Some e \<Rightarrow> Some (subst s1 e)) = Some x" 
-    by auto
-  from S1 S2 Y show "valid_ty_uexpr x" 
-  proof (cases "s2 y")
-    case (Some e)
-    from S1 have "valid_ty_subst s1" by (auto simp add: valid_ty_subst_def ran_def)
-    with S2 Y Some show ?thesis by auto
-  qed auto
-qed
 
 lemma [simp]: "hsubst (combine_subst s t) e = hsubst s (hsubst t e)"
   by (induction e) simp_all
@@ -376,21 +233,26 @@ lemma [simp]: "typecheck' \<Gamma> vs e = (e', t, vs', con) \<Longrightarrow> fi
   by (induction e arbitrary: \<Gamma> vs e' t vs' con) 
      (simp_all add: Let_def split: option.splits prod.splits)
 
-lemma [simp]: "subst_vars \<Gamma> \<subseteq> vs \<Longrightarrow> valid_ty_subst \<Gamma> \<Longrightarrow> t \<in> ran (map_option typeify \<circ> \<Gamma>) \<Longrightarrow> 
-    finite vs \<Longrightarrow> fresh vs \<notin> tvars t"
-  by (unfold subst_vars_def valid_ty_subst_def ran_def) fastforce
-
-lemma [simp]: "typecheck' \<Gamma> vs e = (e', t', vs', con) \<Longrightarrow> x \<in> vs \<Longrightarrow> finite vs \<Longrightarrow>
-  x \<notin> subst_vars \<Gamma> \<Longrightarrow> x \<notin> htvars e'"
+lemma [simp]: "typecheck' \<Gamma> vs e = (e', t', vs', con) \<Longrightarrow> finite vs \<Longrightarrow> htvars e' \<subseteq> vs' - vs"
 proof (induction rule: typecheck_induct)
-  case (NLam \<Gamma> vs vs' con y e\<^sub>1 e\<^sub>1' t' v)
-  moreover hence "x \<notin> subst_vars (\<Gamma>(y \<mapsto> Var v))" by (auto simp add: subst_vars_def ran_def)
-  ultimately show ?case by simp
+  case (NLam \<Gamma> vs vs' con x e\<^sub>1 e\<^sub>1' t' v)
+  moreover hence "insert v vs \<subseteq> vs'" by (metis vars_expand)
+  ultimately show ?case by auto
 next
   case (NApp \<Gamma> vs vs' e\<^sub>1 e\<^sub>2 v e\<^sub>1' t\<^sub>1 vs'' con\<^sub>1 e\<^sub>2' t\<^sub>2 con\<^sub>2)
-  moreover hence "x \<in> vs''" using vars_expand by fastforce
-  ultimately show ?case by simp
+  moreover hence "insert v vs \<subseteq> vs''" by (metis vars_expand)
+  moreover from NApp have "vs'' \<subseteq> vs'" by (metis vars_expand)
+  ultimately show ?case by auto
 qed simp_all
+
+lemma [simp]: "typecheck' \<Gamma> vs e = (e', t', vs', con) \<Longrightarrow> x \<in> vs \<Longrightarrow> finite vs \<Longrightarrow> x \<notin> htvars e'"
+proof -
+  assume "typecheck' \<Gamma> vs e = (e', t', vs', con)"
+     and "finite vs"
+  hence "htvars e' \<subseteq> vs' - vs" by simp
+  moreover assume "x \<in> vs" 
+  ultimately show "x \<notin> htvars e'" by auto
+qed
 
 lemma [simp]: "typecheck' \<Gamma> vs e = (e', t', vs', con) \<Longrightarrow> x \<in> vs \<Longrightarrow> finite vs \<Longrightarrow>
   x \<notin> subst_vars \<Gamma> \<Longrightarrow> x \<notin> vars t'"
@@ -502,43 +364,42 @@ proof (induction "map_option typeify \<circ> \<Gamma>" e\<^sub>t t arbitrary: \<
     con' = con" by (simp add: Let_def)
   from tcn_lam have TV: "tvars t\<^sub>1 \<subseteq> insert ?v vs" by auto
   from tcn_lam have "subst_vars \<Gamma> \<subseteq> insert ?v vs" by auto
-  with TV have X: "subst_vars (\<Gamma>(x \<mapsto> untypify t\<^sub>1)) \<subseteq> insert ?v vs" by simp
-  have Y: "(map_option typeify \<circ> \<Gamma>)(x \<mapsto> t\<^sub>1) = map_option typeify \<circ> (\<Gamma>(x \<mapsto> untypify t\<^sub>1))" by simp
+  with TV have X: "subst_vars (\<Gamma>(x \<mapsto> untypeify t\<^sub>1)) \<subseteq> insert ?v vs" by simp
+  have Y: "(map_option typeify \<circ> \<Gamma>)(x \<mapsto> t\<^sub>1) = map_option typeify \<circ> (\<Gamma>(x \<mapsto> untypeify t\<^sub>1))" by simp
   from tcn_lam have Z: "tvarst e \<subseteq> insert ?v vs" by auto
-  from tcn_lam have W: "valid_ty_subst (\<Gamma>(x \<mapsto> untypify t\<^sub>1))" by simp
-  from tcn_lam T have TC: "typecheck' (\<Gamma>(x \<mapsto> untypify t\<^sub>1)) (insert ?v vs) (erase e) = 
-    (hsubst [?v \<mapsto> untypify t\<^sub>1] e'', subst [?v \<mapsto> untypify t\<^sub>1] t', vs'', 
-      list_subst ?v (untypify t\<^sub>1) con')" by simp
+  from tcn_lam have W: "valid_ty_subst (\<Gamma>(x \<mapsto> untypeify t\<^sub>1))" by simp
+  from tcn_lam T have TC: "typecheck' (\<Gamma>(x \<mapsto> untypeify t\<^sub>1)) (insert ?v vs) (erase e) = 
+    (hsubst [?v \<mapsto> untypeify t\<^sub>1] e'', subst [?v \<mapsto> untypeify t\<^sub>1] t', vs'', 
+      list_subst ?v (untypeify t\<^sub>1) con')" by simp
   from tcn_lam have "finite (insert ?v vs)" by simp
   with tcn_lam X Y Z W TC obtain s where S: "
-    solidify (hsubst s (hsubst [?v \<mapsto> untypify t\<^sub>1] e'')) = e \<and> 
-      typeify (subst s (subst [?v \<mapsto> untypify t\<^sub>1] t')) = t\<^sub>2 \<and>
-        s unifies\<^sub>l list_subst ?v (untypify t\<^sub>1) con' \<and> dom s = vs'' - insert ?v vs \<and> 
+    solidify (hsubst s (hsubst [?v \<mapsto> untypeify t\<^sub>1] e'')) = e \<and> 
+      typeify (subst s (subst [?v \<mapsto> untypeify t\<^sub>1] t')) = t\<^sub>2 \<and>
+        s unifies\<^sub>l list_subst ?v (untypeify t\<^sub>1) con' \<and> dom s = vs'' - insert ?v vs \<and> 
           subst_vars s \<subseteq> tvarst e \<and> valid_ty_subst s \<and> ordered_subst s" by metis
-  from tcn_lam have "subst_vars (\<Gamma>(x \<mapsto> untypify t\<^sub>1)) \<subseteq> vs" by simp
+  from tcn_lam have "subst_vars (\<Gamma>(x \<mapsto> untypeify t\<^sub>1)) \<subseteq> vs" by simp
   moreover from tcn_lam have "?v \<notin> vs" by simp
-  ultimately have "?v \<notin> subst_vars (\<Gamma>(x \<mapsto> untypify t\<^sub>1))" by blast
-  with tcn_lam TC have "?v \<notin> list_vars (list_subst ?v (untypify t\<^sub>1) con')" by simp
+  ultimately have "?v \<notin> subst_vars (\<Gamma>(x \<mapsto> untypeify t\<^sub>1))" by blast
+  with tcn_lam TC have "?v \<notin> list_vars (list_subst ?v (untypeify t\<^sub>1) con')" by simp
   hence "?v \<notin> list_vars con' \<or> ?v \<notin> tvars t\<^sub>1" by (simp split: if_splits)
   from TV S have DV: "dom s \<inter> tvars t\<^sub>1 = {}" by auto
-  with E S have A: "solidify (hsubst (extend_subst ?v (untypify t\<^sub>1) s) e') = TLam x t\<^sub>1 e" 
-    by (simp add: hsubst_merge)
+  with E S have A: "solidify (hsubst (extend_subst ?v (untypeify t\<^sub>1) s) e') = TLam x t\<^sub>1 e" by simp
   from tcn_lam have V: "?v \<notin> tvars t\<^sub>1" by auto
   from S have U: "?v \<notin> dom s" by auto
   from S have "subst_vars s \<subseteq> tvarst e" by simp
   moreover from tcn_lam have "tvarst e \<subseteq> vs \<and> finite vs" by simp
   ultimately have "?v \<notin> subst_vars s" by auto
-  with S V U have B: "ordered_subst (extend_subst ?v (untypify t\<^sub>1) s)" by simp
-  from S E have C: "extend_subst ?v (untypify t\<^sub>1) s unifies\<^sub>l con" by simp
+  with S V U have B: "ordered_subst (extend_subst ?v (untypeify t\<^sub>1) s)" by simp
+  from S E have C: "extend_subst ?v (untypeify t\<^sub>1) s unifies\<^sub>l con" by simp
   from E TC have "insert ?v vs \<subseteq> vs'" by (metis vars_expand)
   with tcn_lam have "insert ?v (vs' - insert ?v vs) = vs' - vs" by auto
-  with S E have D: "dom (extend_subst ?v (untypify t\<^sub>1) s) = vs' - vs" by simp
-  have "vars (subst s (untypify t\<^sub>1)) \<subseteq> vars (untypify t\<^sub>1) - dom s \<union> subst_vars s" 
+  with S E have D: "dom (extend_subst ?v (untypeify t\<^sub>1) s) = vs' - vs" by simp
+  have "vars (subst s (untypeify t\<^sub>1)) \<subseteq> vars (untypeify t\<^sub>1) - dom s \<union> subst_vars s" 
     by (metis vars_subst)
-  with S U have F: "subst_vars (extend_subst ?v (untypify t\<^sub>1) s) \<subseteq> tvarst (TLam x t\<^sub>1 e)" by auto
-  from DV S E have G: "typeify (subst (extend_subst ?v (untypify t\<^sub>1) s) tt) = Arrow t\<^sub>1 t\<^sub>2" 
+  with S U have F: "subst_vars (extend_subst ?v (untypeify t\<^sub>1) s) \<subseteq> tvarst (TLam x t\<^sub>1 e)" by auto
+  from DV S E have G: "typeify (subst (extend_subst ?v (untypeify t\<^sub>1) s) tt) = Arrow t\<^sub>1 t\<^sub>2" 
     by (simp add: subst_merge)
-  from S have "valid_ty_subst (extend_subst ?v (untypify t\<^sub>1) s)" by simp
+  from S have "valid_ty_subst (extend_subst ?v (untypeify t\<^sub>1) s)" by simp
   with A B C D F G show ?case by blast
 next
   case (tcn_app e\<^sub>1 t\<^sub>1 t\<^sub>2 e\<^sub>2)
@@ -554,12 +415,20 @@ next
   with tcn_app TC1 X obtain s\<^sub>1 where S1: "solidify (hsubst s\<^sub>1 e\<^sub>1') = e\<^sub>1 \<and> 
     typeify (subst s\<^sub>1 t\<^sub>1') = Arrow t\<^sub>1 t\<^sub>2 \<and> dom s\<^sub>1 = vs'' - insert ?v vs \<and> subst_vars s\<^sub>1 \<subseteq> tvarst e\<^sub>1 \<and> 
       s\<^sub>1 unifies\<^sub>l con\<^sub>1 \<and> valid_ty_subst s\<^sub>1 \<and> ordered_subst s\<^sub>1" by fastforce
-  from TC1 have V: "insert ?v vs \<subseteq> vs''" by (metis vars_expand)
-  with tcn_app have Y: "subst_vars \<Gamma> \<subseteq> vs''" by auto
-  from tcn_app V have "tvarst e\<^sub>2 \<subseteq> vs''" by auto
+  from TC1 have V1: "insert ?v vs \<subseteq> vs''" by (metis vars_expand)
+  from TC2 E have V2: "vs'' \<subseteq> vs'" by (metis vars_expand)
+  with tcn_app V1 have Y: "subst_vars \<Gamma> \<subseteq> vs''" by auto
+  from tcn_app V1 have "tvarst e\<^sub>2 \<subseteq> vs''" by auto
   with tcn_app TC1 TC2 Y obtain s\<^sub>2 where S2: "solidify (hsubst s\<^sub>2 e\<^sub>2') = e\<^sub>2 \<and> 
     typeify (subst s\<^sub>2 t\<^sub>2') = t\<^sub>1 \<and> dom s\<^sub>2 = vs''' - vs'' \<and> subst_vars s\<^sub>2 \<subseteq> tvarst e\<^sub>2 \<and> 
       s\<^sub>2 unifies\<^sub>l con\<^sub>2 \<and> valid_ty_subst s\<^sub>2 \<and> ordered_subst s\<^sub>2" by fastforce
+
+
+
+
+
+
+
 
 
 
@@ -571,41 +440,79 @@ next
   from tcn_app have "valid_ty_subst \<Gamma>" by simp
 
 
-  from tcn_app S1 S2 have "subst_vars s\<^sub>1 \<subseteq> vs \<and> subst_vars s\<^sub>2 \<subseteq> vs" by auto
+  from tcn_app S1 S2 have SV: "subst_vars s\<^sub>1 \<subseteq> vs \<and> subst_vars s\<^sub>2 \<subseteq> vs" by auto
 
-  from S1 S2 have "dom s\<^sub>1 \<inter> dom s\<^sub>2 = {}" by auto
+  from S1 S2 have DSS: "dom s\<^sub>1 \<inter> dom s\<^sub>2 = {}" by auto
 
 
 
   from tcn_app TC1 S1 have "valid_ty_uexpr t\<^sub>1' \<and> valid_ty_subst s\<^sub>1" by auto
   hence "valid_ty_uexpr (subst s\<^sub>1 t\<^sub>1')" by simp
-  with S1 have "(\<exists>x. t\<^sub>1' = Var x \<and> s\<^sub>1 x = Some (Ctor ''Arrow'' [untypify t\<^sub>1, untypify t\<^sub>2])) \<or>
-    (\<exists>es'. t\<^sub>1' = Ctor ''Arrow'' es' \<and> map (subst s\<^sub>1) es' = [untypify t\<^sub>1, untypify t\<^sub>2])" by auto
+  with S1 have "(\<exists>x. t\<^sub>1' = Var x \<and> s\<^sub>1 x = Some (Ctor ''Arrow'' [untypeify t\<^sub>1, untypeify t\<^sub>2])) \<or>
+    (\<exists>es'. t\<^sub>1' = Ctor ''Arrow'' es' \<and> map (subst s\<^sub>1) es' = [untypeify t\<^sub>1, untypeify t\<^sub>2])" by auto
 
 
-  let ?s = "extend_subst ?v (untypify t\<^sub>2) (combine_subst s\<^sub>1 s\<^sub>2)"
+  from tcn_app have "tvars (Arrow t\<^sub>1 t\<^sub>2) \<subseteq> tvarst e\<^sub>1 \<union> \<Union> (tvars ` ran (map_option typeify \<circ> \<Gamma>))" 
+    by (metis tcn_tvars)
+  with tcn_app have "tvars t\<^sub>1 \<subseteq> tvarst e\<^sub>1 \<union> subst_vars \<Gamma> \<and> tvars t\<^sub>2 \<subseteq> tvarst e\<^sub>1 \<union> subst_vars \<Gamma>" 
+    by (simp add: valid_ty_subst_def subst_vars_def)
+  with tcn_app have VT: "tvars t\<^sub>1 \<subseteq> vs \<and> tvars t\<^sub>2 \<subseteq> vs" by auto
+  hence VUT: "vars (untypeify t\<^sub>1) \<subseteq> vs \<and> vars (untypeify t\<^sub>2) \<subseteq> vs" by simp
 
 
-  have "solidify (hsubst ?s e\<^sub>1') = e\<^sub>1 \<and> solidify (hsubst ?s e\<^sub>2') = e\<^sub>2" by simp
-  hence A: "solidify (hsubst ?s (HApp e\<^sub>1' e\<^sub>2')) = TApp e\<^sub>1 e\<^sub>2" by simp
 
 
-  from S1 S2 E have B: "dom ?s = vs' - vs" by simp
 
 
-  have C: "subst_vars ?s \<subseteq> tvarst (TApp e\<^sub>1 e\<^sub>2)" by simp
+
+  let ?s = "extend_subst ?v (untypeify t\<^sub>2) (combine_subst s\<^sub>1 s\<^sub>2)"
+  from S1 have D1: "dom s\<^sub>1 = vs'' - insert ?v vs" by simp
+  from S2 E have D2: "dom s\<^sub>2 = vs' - vs''" by simp
+  with V1 V2 D1 have D3: "dom (combine_subst s\<^sub>1 s\<^sub>2) = vs' - insert ?v vs" by auto
+  with tcn_app V1 V2 have A: "dom ?s = vs' - vs" by auto
+  from tcn_app TC1 S1 have VS1: "valid_ty_hexpr e\<^sub>1' \<and> valid_ty_subst s\<^sub>1" by auto
+  moreover from S1 have "liquify (solidify (hsubst s\<^sub>1 e\<^sub>1')) = liquify e\<^sub>1" by simp
+  ultimately have H1: "hsubst s\<^sub>1 e\<^sub>1' = liquify e\<^sub>1" by simp
+  from tcn_app TC2 S2 have VS2: "valid_ty_hexpr e\<^sub>2' \<and> valid_ty_subst s\<^sub>2" by auto
+  moreover from S2 have "liquify (solidify (hsubst s\<^sub>2 e\<^sub>2')) = liquify e\<^sub>2" by simp
+  ultimately have H2: "hsubst s\<^sub>2 e\<^sub>2' = liquify e\<^sub>2" by simp
+  from tcn_app have VG: "?v \<notin> subst_vars \<Gamma>" by auto 
+  with tcn_app TC1 have VE1: "?v \<notin> htvars e\<^sub>1'" by simp
+  from tcn_app TC1 TC2 V1 VG have VE2: "?v \<notin> htvars e\<^sub>2'" by simp
+  from tcn_app TC1 have "htvars e\<^sub>1' \<subseteq> vs'' - insert ?v vs" by simp
+  with D2 have HV: "dom s\<^sub>2 \<inter> htvars e\<^sub>1' = {}" by auto
+  from tcn_app have "(vs'' - insert ?v vs) \<inter> tvarst e\<^sub>2 = {}" by auto
+  with S1 H1 H2 VE1 VE2 HV have "solidify (hsubst ?s e\<^sub>1') = e\<^sub>1 \<and> solidify (hsubst ?s e\<^sub>2') = e\<^sub>2" 
+    by simp
+  hence B: "solidify (hsubst ?s (HApp e\<^sub>1' e\<^sub>2')) = TApp e\<^sub>1 e\<^sub>2" by simp
+  from VT D1 have VS1: "tvars t\<^sub>2 \<inter> dom s\<^sub>1 = {}" by auto
+  from V1 VT D2 have VS2: "tvars t\<^sub>2 \<inter> dom s\<^sub>2 = {}" by auto
+  with VS1 have C: "typeify (subst ?s (Var ?v)) = t\<^sub>2" by simp
 
 
-  have D: "?s unifies\<^sub>l con\<^sub>1 @ con\<^sub>2 @ [(t\<^sub>1', Ctor ''Arrow'' [t\<^sub>2', Var ?v])]" by simp
 
 
-  have F: "ordered_subst ?s" by simp
+
+  have TVE: "tvars t\<^sub>2 \<subseteq> tvarst e\<^sub>1 \<union> tvarst e\<^sub>2" by simp
+  from S1 S2 have "subst_vars s\<^sub>1 \<subseteq> tvarst e\<^sub>1 \<union> tvarst e\<^sub>2 \<and> 
+    subst_vars s\<^sub>2 - dom s\<^sub>1 \<subseteq> tvarst e\<^sub>1 \<union> tvarst e\<^sub>2" by blast
+  with DSS D3 VS1 VS2 TVE have D: "subst_vars ?s \<subseteq> tvarst (TApp e\<^sub>1 e\<^sub>2)" by simp
+  from tcn_app SV have VCS: "?v \<notin> subst_vars s\<^sub>1 \<and> (?v \<in> subst_vars s\<^sub>2 \<longrightarrow> ?v \<in> dom s\<^sub>1)" by auto
+  from D2 SV V1 have "dom s\<^sub>2 \<inter> subst_vars s\<^sub>1 = {}" by auto
+  with S1 DSS D3 VCS have UC1: "?s unifies\<^sub>l con\<^sub>1" by simp
+  from S2 D3 VCS DSS have UC2: "?s unifies\<^sub>l con\<^sub>2" by simp
 
 
-  have G: "typeify (subst ?s (Var ?v)) = t\<^sub>2" by simp
+
+  have "subst ?s t\<^sub>1' = Ctor ''Arrow'' [subst ?s t\<^sub>2', subst s\<^sub>1 (subst s\<^sub>2 (untypeify t\<^sub>2))]" by simp
+  with UC1 UC2 have F: "?s unifies\<^sub>l con\<^sub>1 @ con\<^sub>2 @ [(t\<^sub>1', Ctor ''Arrow'' [t\<^sub>2', Var ?v])]" by simp
+                  
 
 
-  have "valid_ty_subst ?s" by simp
+  from D1 D2 VT have "ordered_subst (combine_subst s\<^sub>1 s\<^sub>2) \<and> ?v \<notin> tvars t\<^sub>2 \<and> ?v \<notin> dom s\<^sub>1 \<and> 
+    ?v \<notin> dom s\<^sub>2 \<and> ?v \<notin> subst_vars (combine_subst s\<^sub>1 s\<^sub>2)" by simp
+  hence G: "ordered_subst ?s" by simp
+  from S1 S2 have "valid_ty_subst ?s" by simp
   with E A B C D F G show ?case by blast
 qed auto
 
