02Typed/UnifiableType.thy
@@ -1,0 +1,197 @@
+theory UnifiableType
+  imports Type "../00Utils/Unification/Unification"
+begin
+
+definition env_subst :: "subst \<Rightarrow> subst \<Rightarrow> subst" where
+  "env_subst sub \<Gamma> = map_option (subst sub) \<circ> \<Gamma>"
+
+fun typeify :: "uexpr \<Rightarrow> ty" where
+  "typeify (Var v) = TyVar v"
+| "typeify (Ctor k []) = (if k = ''Base'' then Base else undefined)"
+| "typeify (Ctor k [t\<^sub>1, t\<^sub>2]) = 
+    (if k = ''Arrow'' then Arrow (typeify t\<^sub>1) (typeify t\<^sub>2) else undefined)"
+| "typeify (Ctor k ts) = undefined"
+
+primrec untypeify :: "ty \<Rightarrow> uexpr" where
+  "untypeify (TyVar v) = Var v"
+| "untypeify Base = Ctor ''Base'' []"
+| "untypeify (Arrow t\<^sub>1 t\<^sub>2) = Ctor ''Arrow'' [untypeify t\<^sub>1, untypeify t\<^sub>2]"
+
+fun tsubsts :: "subst \<Rightarrow> ty \<Rightarrow> ty" where
+  "tsubsts sub (TyVar y) = (case sub y of Some t \<Rightarrow> typeify t | None \<Rightarrow> TyVar y)"
+| "tsubsts sub Base = Base"
+| "tsubsts sub (Arrow t\<^sub>1 t\<^sub>2) = Arrow (tsubsts sub t\<^sub>1) (tsubsts sub t\<^sub>2)"
+
+fun valid_ty_uexpr' :: "string \<Rightarrow> nat \<Rightarrow> bool" where
+  "valid_ty_uexpr' k 0 = (k = ''Base'')"
+| "valid_ty_uexpr' k (Suc 0) = False"
+| "valid_ty_uexpr' k (Suc (Suc 0)) = (k = ''Arrow'')"
+| "valid_ty_uexpr' k (Suc (Suc (Suc x))) = False"
+
+primrec valid_ty_uexpr :: "uexpr \<Rightarrow> bool" where
+  "valid_ty_uexpr (Var v) = True"
+| "valid_ty_uexpr (Ctor k ts) = (valid_ty_uexpr' k (length ts) \<and> list_all valid_ty_uexpr ts)"
+
+definition valid_ty_uexprs :: "(uexpr \<times> uexpr) list \<Rightarrow> bool" where
+  "valid_ty_uexprs ts = list_all (\<lambda>(t\<^sub>1, t\<^sub>2). valid_ty_uexpr t\<^sub>1 \<and> valid_ty_uexpr t\<^sub>2) ts"
+ 
+definition valid_ty_subst :: "subst \<Rightarrow> bool" where
+  "valid_ty_subst \<Gamma> = (\<forall>t \<in> ran \<Gamma>. valid_ty_uexpr t)"
+
+lemma [simp]: "typeify (untypeify t) = t"
+  by (induction t) simp_all
+
+lemma [simp]: "valid_ty_uexpr t \<Longrightarrow> untypeify (typeify t) = t"
+  by (induction t rule: typeify.induct) simp_all
+
+lemma [dest]: "typeify e = Arrow t\<^sub>1 t\<^sub>2 \<Longrightarrow> valid_ty_uexpr e \<Longrightarrow> 
+    e = Ctor ''Arrow'' [untypeify t\<^sub>1, untypeify t\<^sub>2]"
+  by (induction e rule: typeify.induct) auto
+
+lemma [simp]: "vars (untypeify t) = tvars t"
+  by (induction t) simp_all
+
+lemma [simp]: "valid_ty_uexpr (untypeify t)"
+  by (induction t) simp_all
+
+lemma [simp]: "valid_ty_uexpr t \<Longrightarrow> tvars (typeify t) = vars t"
+  by (induction t rule: typeify.induct) simp_all
+
+lemma [simp]: "tsubsts Map.empty e = e"
+  by (induction e) simp_all
+
+lemma [simp]: "dom s \<inter> tvars t = {} \<Longrightarrow> tsubsts s t = t"
+  by (induction t) (auto split: option.splits)
+
+lemma [simp]: "valid_ty_uexpr t \<Longrightarrow> typeify (subst sub t) = tsubsts sub (typeify t)"
+  by (induction t rule: typeify.induct) (simp_all split: option.splits)
+
+lemma [simp]: "valid_ty_subst sub \<Longrightarrow> untypeify (tsubsts sub t) = subst sub (untypeify t)"
+  by (induction t) (auto simp add: valid_ty_subst_def ran_def split: option.splits)
+
+lemma valid_empty [simp]: "valid_ty_subst Map.empty"
+  by (simp add: valid_ty_subst_def)
+
+lemma [simp]: "valid_ty_uexpr e \<Longrightarrow> typeify (subst sub e) = tsubsts sub (typeify e)"
+  by (induction e rule: typeify.induct) (auto split: option.splits)
+
+lemma [simp]: "valid_ty_subst \<Gamma> \<Longrightarrow> 
+    map_option (typeify \<circ> subst sub) (\<Gamma> x) = map_option (tsubsts sub \<circ> typeify) (\<Gamma> x)"
+  by (cases "\<Gamma> x") (auto simp add: valid_ty_subst_def ran_def)
+
+lemma [simp]: "valid_ty_subst \<Gamma> \<Longrightarrow> 
+    map_option (typeify \<circ> subst sub) \<circ> \<Gamma> = map_option (tsubsts sub \<circ> typeify) \<circ> \<Gamma>"
+  by auto
+
+lemma [simp]: "valid_ty_subst \<Gamma> \<Longrightarrow> valid_ty_uexpr t \<Longrightarrow> valid_ty_subst (\<Gamma>(x \<mapsto> t))"
+  by (auto simp add: valid_ty_subst_def ran_def)
+
+lemma [simp]: "valid_ty_subst \<Gamma> \<Longrightarrow> valid_ty_subst \<Gamma>' \<Longrightarrow> valid_ty_subst (\<Gamma>(x := \<Gamma>' y))"
+  by (auto simp add: valid_ty_subst_def ran_def)
+
+lemma [simp]: "valid_ty_uexpr e \<Longrightarrow> valid_ty_uexpr e' \<Longrightarrow> valid_ty_uexpr (subst [x \<mapsto> e'] e)"
+  and [simp]: "list_all valid_ty_uexpr es \<Longrightarrow> valid_ty_uexpr e' \<Longrightarrow> 
+    list_all valid_ty_uexpr (map (subst [x \<mapsto> e']) es)"
+proof (induction e and es rule: vars_varss.induct)
+  case (2 k es)
+  thus ?case 
+  proof (induction es)
+    case (Cons a es)
+    thus ?case 
+    proof (induction es)
+      case (Cons b es)
+      thus ?case by (induction es) simp_all
+    qed simp_all
+  qed simp_all
+qed simp_all
+
+lemma [simp]: "valid_ty_uexpr e \<Longrightarrow> valid_ty_uexprs ess \<Longrightarrow> valid_ty_uexprs (list_subst x e ess)"
+  by (induction ess rule: list_subst.induct) (auto simp add: valid_ty_uexprs_def)
+
+lemma [simp]: "valid_ty_uexpr t \<Longrightarrow> valid_ty_subst sub \<Longrightarrow> valid_ty_uexpr (subst sub t)"
+  and [simp]: "list_all valid_ty_uexpr ts \<Longrightarrow> valid_ty_subst sub \<Longrightarrow> 
+    list_all valid_ty_uexpr (map (subst sub) ts)"
+  by (induction t and ts rule: vars_varss.induct) 
+     (auto simp add: valid_ty_subst_def ran_def split: option.splits)
+
+lemma [simp]: "valid_ty_subst s \<Longrightarrow> valid_ty_uexpr e \<Longrightarrow> valid_ty_subst (extend_subst x e s)"
+  by (auto simp add: valid_ty_subst_def extend_subst_def ran_def)
+
+lemma [elim]: "valid_ty_subst \<Gamma> \<Longrightarrow> \<Gamma> x = Some t \<Longrightarrow> valid_ty_uexpr t"
+  by (auto simp add: valid_ty_subst_def ran_def)
+
+lemma [simp]: "valid_ty_subst \<Gamma> \<Longrightarrow> valid_ty_subst sub\<^sub>2 \<Longrightarrow> 
+  map_option (typeify \<circ> subst sub\<^sub>1 \<circ> subst sub\<^sub>2) (\<Gamma> x) = 
+    map_option (tsubsts sub\<^sub>1 \<circ> tsubsts sub\<^sub>2 \<circ> typeify) (\<Gamma> x)"
+proof (cases "\<Gamma> x")
+  case (Some e)
+  moreover assume "valid_ty_subst \<Gamma>"
+  ultimately have E: "valid_ty_uexpr e" by auto
+  assume "valid_ty_subst sub\<^sub>2"
+  with Some E show ?thesis by simp
+qed simp_all
+
+lemma [simp]: "valid_ty_subst \<Gamma> \<Longrightarrow> valid_ty_subst sub\<^sub>2 \<Longrightarrow> 
+  map_option (typeify \<circ> subst sub\<^sub>1 \<circ> subst sub\<^sub>2) \<circ> \<Gamma> = 
+    map_option (tsubsts sub\<^sub>1 \<circ> tsubsts sub\<^sub>2 \<circ> typeify) \<circ> \<Gamma>"
+  by auto
+
+lemma [elim]: "valid_ty_uexprs ts \<Longrightarrow> unify' ts = Some sub \<Longrightarrow> valid_ty_subst sub"                                  
+proof (induction ts arbitrary: sub rule: unify'.induct)
+  case (2 k\<^sub>1 es\<^sub>1 k\<^sub>2 es\<^sub>2 ess)
+  moreover hence "list_all valid_ty_uexpr es\<^sub>1" by (auto simp add: valid_ty_uexprs_def)
+  moreover from 2 have "list_all valid_ty_uexpr es\<^sub>2" by (auto simp add: valid_ty_uexprs_def)
+  ultimately show ?case by (simp add: valid_ty_uexprs_def split: if_splits)
+next
+  case (4 x e ess)
+  thus ?case
+  proof (cases "e = Var x")
+    case False note F = False
+    with 4 show ?thesis 
+    proof (cases "x \<in> vars e")
+      case False
+      with 4 F obtain sub' where S: "unify' (list_subst x e ess) = Some sub' \<and> 
+        sub = extend_subst x e sub'" by auto
+      from 4 have "valid_ty_uexpr e \<and> valid_ty_uexprs ess" by (simp add: valid_ty_uexprs_def)
+      hence "valid_ty_uexprs (list_subst x e ess)" by simp
+      with 4 F False S show ?thesis by (simp add: valid_ty_uexprs_def)
+    qed simp_all
+  qed (simp_all add: valid_ty_uexprs_def)
+qed (auto simp add: valid_ty_uexprs_def)
+
+lemma [elim]: "valid_ty_uexpr t\<^sub>1 \<Longrightarrow> valid_ty_uexpr t\<^sub>2 \<Longrightarrow> unify t\<^sub>1 t\<^sub>2 = Some sub \<Longrightarrow> 
+  valid_ty_subst sub"                                  
+proof (unfold unify_def)
+  assume "valid_ty_uexpr t\<^sub>1" and "valid_ty_uexpr t\<^sub>2" 
+  hence "valid_ty_uexprs [(t\<^sub>1, t\<^sub>2)]" by (simp add: valid_ty_uexprs_def)
+  moreover assume "unify' [(t\<^sub>1, t\<^sub>2)] = Some sub"
+  ultimately show "valid_ty_subst sub" by auto
+qed
+
+lemma valid_ty_uexpr_structrual [simp]: "structural valid_ty_uexpr"
+  by (auto simp add: structural_def)
+
+lemma [simp]: "valid_ty_subst sub \<Longrightarrow> valid_ty_subst \<Gamma> \<Longrightarrow> valid_ty_subst (env_subst sub \<Gamma>)"
+  by (auto simp add: valid_ty_subst_def env_subst_def ran_def)
+
+lemma [simp]: "valid_ty_subst s1 \<Longrightarrow> valid_ty_subst s2 \<Longrightarrow> valid_ty_subst (combine_subst s1 s2)"
+proof (unfold valid_ty_subst_def combine_subst_def ran_def, rule)
+  fix x
+  assume S1: "\<forall>x \<in> {b. \<exists>a. s1 a = Some b}. valid_ty_uexpr x"
+  assume S2: "\<forall>x \<in> {b. \<exists>a. s2 a = Some b}. valid_ty_uexpr x"
+  assume "x \<in> {b. \<exists>a. (case s2 a of None \<Rightarrow> s1 a | Some e \<Rightarrow> Some (subst s1 e)) = Some b}"
+  then obtain y where Y: "(case s2 y of None \<Rightarrow> s1 y | Some e \<Rightarrow> Some (subst s1 e)) = Some x" 
+    by auto
+  from S1 S2 Y show "valid_ty_uexpr x" 
+  proof (cases "s2 y")
+    case (Some e)
+    from S1 have "valid_ty_subst s1" by (auto simp add: valid_ty_subst_def ran_def)
+    with S2 Y Some show ?thesis by auto
+  qed auto
+qed
+
+lemma [simp]: "subst_vars \<Gamma> \<subseteq> vs \<Longrightarrow> valid_ty_subst \<Gamma> \<Longrightarrow> t \<in> ran (map_option typeify \<circ> \<Gamma>) \<Longrightarrow> 
+    finite vs \<Longrightarrow> fresh vs \<notin> tvars t"
+  by (unfold subst_vars_def valid_ty_subst_def ran_def) fastforce
+
+end
